implem universes graph

template-coq/src/ast_quoter.ml
@@ -21,7 +21,7 @@ struct
   type quoted_proj = projection
   type quoted_global_reference = global_reference
 
-  type quoted_sort_family = sort_family
+  type quoted_sort_family = Universes0.sort_family
   type quoted_constraint_type = Universes0.constraint_type
   type quoted_univ_constraint = Universes0.univ_constraint
   type quoted_univ_instance = Universes0.Instance.t
@@ -78,9 +78,9 @@ struct
 
   let quote_sort_family s =
     match s with
-    | Sorts.InProp -> BasicAst.InProp
-    | Sorts.InSet -> BasicAst.InSet
-    | Sorts.InType -> BasicAst.InType
+    | Sorts.InProp -> Universes0.InProp
+    | Sorts.InSet -> Universes0.InSet
+    | Sorts.InType -> Universes0.InType
 
   let quote_cast_kind = function
     | DEFAULTcast -> Cast
@@ -337,16 +337,15 @@ struct
   let unquote_level_expr (trm : Universes0.Level.t) (b : quoted_bool) : Univ.Universe.t =
     let l = unquote_level trm in
     let u = Univ.Universe.make l in
-    if b then Univ.Universe.super u
+    if b && not (Univ.Level.is_prop l) then Univ.Universe.super u
     else u
 
   let unquote_universe evd (trm : Universes0.Universe.t) =
-    match Specif.projT1 trm with
-    | [] -> Evd.new_univ_variable (Evd.UnivFlexible false) evd
-    | (l,b)::q ->
-      evd, List.fold_left (fun u (l,b) ->
-          let u' = unquote_level_expr l b in Univ.Universe.sup u u')
-        (unquote_level_expr l b) q
+    (* | [] -> Evd.new_univ_variable (Evd.UnivFlexible false) evd *)
+    let rec aux = function
+      | Utils.NEL.Coq_sing (l,b) -> unquote_level_expr l b
+      | Utils.NEL.Coq_cons ((l,b), q) -> Univ.Universe.sup (aux q) (unquote_level_expr l b)
+    in evd, aux trm
 
   let quote_global_reference : Globnames.global_reference -> quoted_global_reference = function
     | Globnames.VarRef _ -> CErrors.user_err (Pp.str "VarRef unsupported")
